theories/lang/cpp/syntax/typing.v
@@ -1,5 +1,5 @@
 (*
- * Copyright (c) 2020 BedRock Systems, Inc.
+ * Copyright (c) 2020-2023 BedRock Systems, Inc.
  * This software is distributed under the terms of the BedRock Open-Source License.
  * See the LICENSE-BedRock file in the repository root for details.
  *)
@@ -27,18 +27,18 @@ Fixpoint type_of (e : Expr) : type :=
   | Epostdec _ t => t
   | Eseqand _ _ => Tbool
   | Eseqor _ _ => Tbool
-  | Ecomma _ _ e2 => type_of e2
+  | Ecomma _ e2 => type_of e2
   | Ecall _ _ t
   | Ecast _ _ _ t
-  | Emember _ _ _ t
-  | Emember_call _ _ _ _ t
-  | Esubscript _ _ t
+  | Emember _ _ t
+  | Emember_call _ _ _ t
+  | Esubscript _ _ _ t
   | Esize_of _ t
   | Ealign_of _ t
   | Eoffset_of _ t
   | Econstructor _ _ t => t
   | Eimplicit e => type_of e
-  | Eif _ _ _ t
+  | Eif _ _ _ _ t
   | Ethis t => t
   | Enull => Tnullptr
   | Einitlist _ _ t
@@ -46,15 +46,14 @@ Fixpoint type_of (e : Expr) : type :=
   | Enew _ _ aty _ _ => Tptr aty
   | Edelete _ _ _ _ => Tvoid
   | Eandclean e => type_of e
-  | Ematerialize_temp e => type_of e
-  | Ebuiltin _ t => t
+  | Ematerialize_temp e _ => type_of e
   | Eatomic _ _ t => t
   | Eva_arg _ t => t
   | Epseudo_destructor _ _ => Tvoid
-  | Earrayloop_init _ _ _ _ _ _ t => t
+  | Earrayloop_init _ _ _ _ _ t => t
   | Earrayloop_index _ t => t
-  | Eopaque_ref _ t => t
-  | Eunsupported _ t => t
+  | Eopaque_ref _ _ t => t
+  | Eunsupported _ _ t => t
   end.
 
 (** [erase_qualifiers t] erases *all* qualifiers that occur everywhere in the type.
@@ -188,3 +187,133 @@ Definition is_value_type (t : type) : bool :=
   | Tvoid => true
   | _ => false
   end.
+
+(**
+Setting aside uninstantiated template arguments, there's a total
+function from expressions to value categories.
+*)
+Definition UNEXPECTED_valcat {A} (tm : A) : ValCat.
+Proof. exact Prvalue. Qed.
+
+(**
+The value category of an explicit cast to type [t] or a call to a
+function returning type [t] or a [__builtin_va_arg] of type [t].
+*)
+Definition valcat_from_type (t : type) : ValCat :=
+  (*
+  Dropping qualifiers may not be necessary. Cppreference says
+  "Reference types cannot be cv-qualified at the top level".
+  *)
+  match drop_qualifiers t with
+  | Tref _
+  | Trv_ref (@Tfunction _ _ _ _) => Lvalue
+  | Trv_ref _ => Xvalue
+  | _ => Prvalue
+  end.
+
+Definition valcat_from_function_type (t : type) : ValCat :=
+  match t with
+  | @Tfunction _ _ ret _ => valcat_from_type ret
+  | _ => UNEXPECTED_valcat t
+  end.
+
+Fixpoint valcat_of (e : Expr) : ValCat :=
+  match e with
+  | Econst_ref _ _ => Prvalue
+  | Evar _ _ => Lvalue
+  | Echar _ _ => Prvalue
+  | Estring _ _ => Lvalue
+  | Eint _ _ => Prvalue
+  | Ebool _ => Prvalue
+  | Eunop _ _ _ => Prvalue
+  | Ebinop op e1 _ _ =>
+    match op with
+    | Bdotp =>
+      (**
+      The value category of [e1.*e2] is (i) that of [e1] (xvalue or
+      lvalue) when [e2] points to a field and (ii) prvalue when [e2]
+      points to a method.
+
+      We need only address (i) here because when [e2] is a method, the
+      result of [e1.*e2] must be immediately applied, and cpp2v emits
+      [Emember_call] rather than [Ebinop] for indirect method calls.
+
+      https://www.eel.is/c++draft/expr.mptr.oper#6
+      *)
+      match e1 with
+      | Eread_ref _ => Lvalue
+      | Ematerialize_temp _ _ => Xvalue
+      | _ => UNEXPECTED_valcat e
+      end
+    | Bdotip => Lvalue	(* derived from [Bdotp] *)
+    | _ => Prvalue
+    end
+  | Eread_ref e =>
+    (*
+    cpp2v ensures [e] is either a variable [Evar] or a field [Emember]
+    with reference type. According to cppreference, "the name of a
+    variable, [...], or a data member, regardless of type" is an
+    lvalue.
+    *)
+    Lvalue
+  | Ederef _ _ => Lvalue
+  | Eaddrof _ => Prvalue
+  | Eassign _ _ _ => Lvalue
+  | Eassign_op _ _ _ _ => Lvalue
+  | Epreinc _ _ => Lvalue
+  | Epostinc _ _ => Prvalue
+  | Epredec _ _ => Lvalue
+  | Epostdec _ _ => Prvalue
+  | Eseqand _ _ => Prvalue
+  | Eseqor _ _ => Prvalue
+  | Ecomma _ e2 => valcat_of e2
+  | Ecast _ _ vc _ => vc
+  | Ecall f _ _ =>
+    match f with
+    | Ecast Cfun2ptr _ _ (Tptr t) => valcat_from_function_type t
+    | _ => UNEXPECTED_valcat e
+    end
+  | Emember e _ _ => valcat_of e
+  | Emember_call f _ _ _ =>
+    match f with
+    | inl (_, _, t)
+    | inr (Ecast Cl2r _  _ (Tmember_pointer _ t)) => valcat_from_function_type t
+    | _ => UNEXPECTED_valcat e
+    end
+  | Esubscript _ _ vc _ => vc
+  | Esize_of _ _ => Prvalue
+  | Ealign_of _ _ => Prvalue
+  | Eoffset_of _ _ => Prvalue
+  | Econstructor _ _ _ => Prvalue (* init *)
+  | Eimplicit e => valcat_of e
+  | Eif _ e1 e2 vc _ => vc
+  | Ethis _ => Prvalue
+  | Enull => Prvalue
+  | Einitlist _ _ t => Prvalue (* operand | init *)
+  | Eimplicit_init _ =>
+    (**
+    "References cannot be value-initialized".
+
+    https://en.cppreference.com/w/cpp/language/value_initialization
+    *)
+    Prvalue
+  | Enew _ _ _ _ _ => Prvalue
+  | Edelete _ _ _ _ => Prvalue
+  | Eandclean e => valcat_of e
+  | Ematerialize_temp _ vc => vc
+  | Eatomic _ _ _ => Prvalue
+  | Eva_arg _ t => valcat_from_type t
+  | Epseudo_destructor _ _ => Prvalue
+  | Earrayloop_init _ _ _ _ _ _ => Prvalue (* init *)
+  | Earrayloop_index _ _ => Prvalue
+  | Eopaque_ref _ vc _ => vc
+  | Eunsupported _ vc _ => vc
+  end.
+#[global] Arguments valcat_of !_ / : simpl nomatch, assert.
+
+Definition vctype_of (e : Expr) : type :=
+  match valcat_of e with
+  | Prvalue => id
+  | Lvalue => Tref
+  | Xvalue => Trv_ref
+  end (type_of e).
